Denotational.thy
@@ -1,0 +1,198 @@
+theory Denotational
+  imports Terms Heap "~~/src/HOL/HOLCF/HOLCF"
+begin
+
+default_sort cpo
+
+instantiation var :: discrete_cpo
+begin
+  definition  [simp]: "(x::var) \<sqsubseteq> y \<longleftrightarrow> x = y"
+  instance by default simp
+end
+
+class cont_pt = 
+  cpo + 
+  pt +
+  assumes perm_cont: "\<And>p. cont ((permute p) :: 'a::{cpo,pt} \<Rightarrow> 'a)"
+
+lemmas perm_cont2cont[simp,cont2cont] = cont_compose[OF perm_cont]
+
+instance var :: cont_pt  by default auto
+
+instantiation "cfun" :: (cont_pt, cont_pt) pt
+begin
+  definition "p \<bullet> (f :: 'a  \<rightarrow> 'b) = (\<Lambda> x. p \<bullet> (f \<cdot> (- p \<bullet> x)))"
+
+  instance
+  apply(default)
+  apply (simp add: permute_cfun_def eta_cfun)
+  apply (simp add: permute_cfun_def cfun_eqI minus_add)
+  done
+end
+
+class pure_cpo = Nominal2_Base.pure + cpo
+
+instance pure_cpo \<subseteq> cont_pt
+  apply default
+  proof-
+    fix p :: perm
+    have "permute p = ((\<lambda>x. x) :: 'a \<Rightarrow> 'a)" by(rule)(rule permute_pure)
+    thus "cont (permute p :: 'a \<Rightarrow> 'a)" by (auto)
+  qed
+
+instance "cfun" :: (pure_cpo, pure_cpo) pure_cpo
+  apply default
+  apply (auto  simp add: permute_cfun_def permute_pure Cfun.cfun.Rep_cfun_inverse)
+  done
+
+definition cfun_upd :: "('a \<rightarrow> 'b) => 'a => 'b => ('a \<rightarrow> 'b)" where
+  "cfun_upd f a b == \<Lambda> x. if x=a then b else f\<cdot>x"
+
+nonterminal cupdbinds and cupdbind
+
+syntax
+  "_cupdbind" :: "['a, 'a] => cupdbind"               ("(2_ :\<cdot>=/ _)")
+  ""         :: "cupdbind => cupdbinds"               ("_")
+  "_cupdbinds":: "[cupdbind, cupdbinds] => cupdbinds" ("_,/ _")
+  "_cUpdate"  :: "['a, cupdbinds] => 'a"              ("_/'((_)')" [1000, 0] 900)
+
+translations
+  "_cUpdate f (_cupdbinds b bs)" == "_cUpdate (_cUpdate f b) bs"
+  "f(x:\<cdot>=y)" == "CONST cfun_upd f x y"
+
+find_theorems cont "if _ then _ else _ "
+
+
+lemma cfun_upd_eqvt[eqvt]: "p \<bullet> (cfun_upd f (x::'a::{cont_pt,discrete_cpo}) y) = cfun_upd (p \<bullet> f) (p \<bullet> x) (p \<bullet> y)"
+using [[show_sorts]]
+by (auto simp add:permute_cfun_def cfun_eq_iff cfun_upd_def)
+
+domain Value = Fn (lazy "Value \<rightarrow> Value")
+
+fixrec Fn_project :: "Value \<rightarrow> Value \<rightarrow> Value" (* (infix "\<down>Fn" 70) *)
+ where "Fn_project\<cdot>(Fn\<cdot>f)\<cdot>v = f \<cdot> v"
+
+abbreviation Fn_project_abbr (infix "\<down>Fn" 55)
+  where "f \<down>Fn v \<equiv> Fn_project\<cdot>f\<cdot>v"
+
+lemma "Fn\<cdot>(\<Lambda> x . \<bottom>) \<noteq> \<bottom>" by simp
+
+type_synonym Env = "var \<rightarrow> Value"
+
+instantiation Value :: pure_cpo
+begin
+  definition "p \<bullet> (v::Value) = v"
+instance
+  apply default
+  apply (auto simp add: permute_Value_def)
+  done
+end
+
+function heapToEnv :: "heap \<Rightarrow> (exp \<Rightarrow> Value)  \<Rightarrow> Env"
+where
+  "heapToEnv [] _ = \<bottom>"
+| "heapToEnv ((x,e)#h) eval = (heapToEnv h eval) (x :\<cdot>= eval e)"
+by (pat_completeness, auto)
+termination by lexicographic_order
+
+nominal_primrec
+  ESem :: "exp \<Rightarrow> Env \<Rightarrow> Value" ("\<lbrakk> _ \<rbrakk>\<^bsub>_\<^esub>"  [60,60] 60)
+and
+  HSem :: "heap => Env => Env" ("\<lbrace> _ \<rbrace>_"  [60,60] 60) 
+where
+  "atom x \<sharp> \<rho> ==> \<lbrakk> Lam [x]. e \<rbrakk>\<^bsub>\<rho>\<^esub> = Fn \<cdot> (\<Lambda> v. (\<lbrakk> e \<rbrakk>\<^bsub>\<rho>(x :\<cdot>= v)\<^esub>))"
+| "\<lbrakk> App e x \<rbrakk>\<^bsub>\<rho>\<^esub> = \<lbrakk> e \<rbrakk>\<^bsub>\<rho>\<^esub> \<down>Fn \<lbrakk> Var x \<rbrakk>\<^bsub>\<rho>\<^esub> "
+| "\<lbrakk> Var x \<rbrakk>\<^bsub>\<rho>\<^esub> = \<rho>\<cdot>x"
+| "\<lbrakk> Let as body\<rbrakk>\<^bsub>\<rho>\<^esub> = \<lbrakk> Let as body\<rbrakk>\<^bsub>\<lbrace> asToHeap as \<rbrace>\<rho>\<^esub>"
+| "\<lbrace> h \<rbrace>\<rho> = (\<mu> \<rho>'. lub{\<rho>, heapToEnv h (\<lambda> e . \<lbrakk>e\<rbrakk>\<^bsub>\<rho>'\<^esub>)})"
+proof-
+have eqvt_at_ESem: "\<And> a b . eqvt_at ESem_HSem_sumC (Inl (a, b)) \<Longrightarrow> eqvt_at (\<lambda>(a, b). ESem a b) (a, b)" sorry
+have eqvt_at_HSem: "\<And> a b . eqvt_at ESem_HSem_sumC (Inr (a, b)) \<Longrightarrow> eqvt_at (\<lambda>(a, b). HSem a b) (a, b)" sorry
+
+{
+
+case goal1 thus ?case
+  unfolding eqvt_def ESem_HSem_graph_def
+  apply rule
+  apply perm_simp
+  sorry (* :-( *)
+
+(* Exhaustiveness *)
+next
+case (goal3 P x) 
+  show ?case
+  proof(cases x)
+    case (Inl a)
+      show ?thesis
+      proof(cases a)
+        case (Pair e \<rho>)
+          show ?thesis 
+          using Pair Inl goal3
+          apply (rule_tac y=e in exp_assn.exhaust(1))
+          apply auto[1]
+          apply blast
+          apply blast
+          using [[show_sorts]]
+          apply (rule_tac y=e and c = \<rho> in exp_assn.strong_exhaust(1))
+          
+          
+          
+          thm exp_assn.strong_exhaust(1)
+          proof(cases e P rule: exp_assn.strong_exhaust(1))
+            case (goal1 v) thus ?thesis using  Inl Pair goal3(3) by auto next
+            case (goal2 e x) thus ?thesis using  Inl Pair goal3(2) by auto next
+            case goal3 thus ?thesis using  Inl Pair goal3(2) by auto next
+          using Pair Inl goal3
+
+
+          apply simp
+  apply(case_tac x)
+  apply(case_tac a)
+  thm exp_assn.strong_exhaust(1)
+  apply(rule_tac y = aa and c = ba in exp_assn.strong_exhaust(1), (auto simp add:fresh_star_def))[1]
+  (* 
+  apply(case_tac b)
+  apply(case_tac a)
+  *)
+  apply auto
+  sorry
+
+next
+case (goal4 x \<rho> e x' \<rho>' e')
+  have eqvt1: "(\<And>xa. eqvt_at (\<lambda>(a, b). ESem a b) (e, \<rho>(x :\<cdot>= xa)))" using goal4 by -(rule eqvt_at_ESem)
+  have eqvt2: "(\<And>xa. eqvt_at (\<lambda>(a, b). ESem a b) (e', \<rho>'(x' :\<cdot>= xa)))"  using goal4 by -(rule eqvt_at_ESem)
+
+  have tmp2: "[[atom x]]lst. e = [[atom x']]lst. e'" and rho_eq:"\<rho> = \<rho>'"  using goal4(7) by auto  
+
+  thm Abs_lst1_fcb[OF tmp2]
+
+  have all_fresh: "(atom x' \<rightleftharpoons> atom x) \<bullet> \<rho>' = \<rho>'" 
+    using goal4 `\<rho> = \<rho>'`
+    by (auto simp add: swap_fresh_fresh)
+
+  have tmp: "\<And> xa. ESem e (\<rho>(x :\<cdot>= xa)) = ESem e' (\<rho>'(x' :\<cdot>= xa))"
+    using eqvt1 eqvt2 tmp2 rho_eq goal4(5) goal4(6)
+    using [[show_types]]
+    apply (simp add: Abs1_eq_iff')
+    apply auto
+
+    apply (erule_tac x = xa in meta_allE)
+    apply (erule_tac x = xa in meta_allE)
+    apply (simp only: eqvt_at_def)
+    apply auto
+
+    apply (erule_tac x = "(atom x' \<rightleftharpoons> atom x)" in allE)
+    apply (auto simp add: cfun_upd_eqvt permute_Value_def all_fresh)
+    done
+
+
+   show ?case
+    apply (simp only: meta_eq_to_obj_eq[OF ESem_def, symmetric, unfolded fun_eq_iff]
+      meta_eq_to_obj_eq[OF HSem_def, symmetric, unfolded fun_eq_iff])
+    (* No _sum any more at this point! *)
+    by (auto simp add: tmp)
+next
+ 
+apply_end(auto)
+
+end
