Heap.thy
@@ -1,0 +1,34 @@
+theory Heap
+imports Terms
+begin
+
+type_synonym heap = "(var \<times> exp) list"
+
+definition heapVars
+  where "heapVars h = fst ` set h"
+
+lemma [simp]:"heapVars (a @ b) = heapVars a \<union> heapVars b"
+  and [simp]:"heapVars ((v,e) # h) = insert v (heapVars h)"
+  by (auto simp add: heapVars_def)
+
+nominal_primrec  asToHeap :: "assn \<Rightarrow> heap" 
+ where ANilToHeap: "asToHeap ANil = []"
+ | AConsToHeap: "asToHeap (ACons v e as) = (v, e) # asToHeap as"
+unfolding eqvt_def asToHeap_graph_def
+apply rule
+apply perm_simp
+apply rule
+apply rule
+apply(case_tac x rule: exp_assn.exhaust(2))
+apply auto
+done
+termination(eqvt) by lexicographic_order
+
+lemmas asToHeap_induct = asToHeap.induct[case_names ANilToHeap AConsToHeap]
+
+lemma asToHeap_eqvt[eqvt]:
+ fixes \<pi>::perm
+ shows "\<pi> \<bullet> (asToHeap as) = asToHeap (\<pi> \<bullet> as)"
+by(induct as rule:asToHeap.induct) (auto)
+
+end
